cakeml_connection/opentheory-reader/readerVerilogProofScript.sml
@@ -1,3 +1,5 @@
+open wordsLib; (* Must be loaded before readerProgProofTheory? Why? *)
+
 open hardwarePreamble;
 
 open readerProgProofTheory;
@@ -7,6 +9,136 @@ open commonVerilogProofLib;
 
 val _ = new_theory "readerVerilogProof";
 
-(* TODO *)
+val _ = Parse.hide "mem";
+val mem = ``mem:'U->'U-> bool``;
+val _ = temp_overload_on ("reader", ``\inp r. readLines inp init_state r``);
+
+val reader_spec_def = Define `
+ reader_spec mem input cl stdout stderr <=>
+  let refs = SND (init_reader () init_refs) in
+   case reader (lines_of (implode input)) refs of
+     (Failure (Fail e), refs) => (stdout = "") /\ (stderr = explode e)
+   | (Success (s, _), refs) =>
+      (is_set_theory ^mem ==>
+       (!asl c. MEM (Sequent asl c) s.thms ==> (thyof refs.the_context, asl) |= c)) /\
+     refs.the_context extends init_ctxt /\
+     (stdout = explode (msg_success s refs.the_context)) /\ (stderr = "")
+   | _ => F`;
+
+val reader_cl_ok_def = Define `
+ reader_cl_ok cl <=>
+  wfcl cl ∧
+  SUM (MAP strlen cl) + LENGTH cl ≤ cline_size ∧
+  (LENGTH cl = 1)`;
+
+val reader_ag32_next_verilog = Q.prove(
+ `!vstep fext ms mem cl input.
+   vstep = verilog_sem fext computer ms ∧
+
+   reader_cl_ok cl ∧
+   STRLEN input ≤ stdin_size ∧
+
+   is_lab_env fext_accessor_verilog vstep fext ∧
+   ag32_verilog_init (code, data, config) (cl, input) ms fext
+   ⇒
+   ?stdout stderr k1. !k. k1 ≤ k ==> ?fin.
+    reader_spec ^mem input cl stdout stderr /\
+    vstep k = INR fin /\
+    let outs = MAP get_ag32_io_event (fext k).io_events;
+        outs_stdout = extract_writes 1 outs;
+        outs_stderr = extract_writes 2 outs
+    in
+      is_halted (code, data, config) fin ∧
+      outs_stdout ≼ stdout ∧
+      outs_stderr ≼ stderr ∧
+      (exit_code_0 fin ⇒
+       outs_stdout = stdout ∧
+       outs_stderr = stderr)`,
+ rewrite_tac [reader_cl_ok_def, reader_spec_def] \\
+ (* Hack for now, use lift_tac later *)
+ rewrite_tac [verilog_sem_def] \\ rpt gen_tac \\
+ SELECT_ELIM_TAC \\ conj_asm1_tac >- metis_tac[lift_fext_exists] \\
+ pop_assum strip_assume_tac \\
+
+ rewrite_tac [ag32_verilog_init_def] \\ rpt strip_tac \\ last_x_assum kall_tac \\
+ drule_strip (vars_has_type_append |> SPEC_ALL |> EQ_IMP_RULE |> fst |> SPEC_ALL) \\
+(*
+ rewrite_tac [ag32_verilog_init_def] \\ rpt strip_tac \\
+ `mrun x computer ms = mrun x' computer ms` by metis_tac [lift_fext_unique] \\
+ last_x_assum kall_tac \\ FULL_SIMP_TAC bool_ss [] \\ pop_assum kall_tac \\
+ drule_strip (vars_has_type_append |> SPEC_ALL |> EQ_IMP_RULE |> fst |> SPEC_ALL) \\
+*)
+
+ (* Instantiate output etc. *) (* <-- modified *)
+ simp [] \\
+ qmatch_goalsub_abbrev_tac `pair_CASE res _` \\
+ qexists_tac `case res of
+               (Success (s,v11),refs) => explode (msg_success s refs.the_context)
+               | _ => ""` \\
+ qexists_tac `case res of
+               (Failure (Fail e), _) => explode e
+               | _ => ""` \\
+
+ drule_strip relM_backwards \\
+ drule_strip INIT_backwards \\
+ qmatch_asmsub_abbrev_tac `INIT _ _ s'` \\
+
+ (* modified: *)
+ drule_strip (reader_ag32_next |> GEN_ALL) \\
+
+ disch_then (qspec_then `s'` mp_tac) \\
+ impl_tac >- (qunabbrev_tac `s'` \\ simp [ag32_targetTheory.is_ag32_init_state_def]) \\
+
+ strip_tac \\
+ first_x_assum(qspec_then`k1`mp_tac) \\
+ impl_tac >- simp[] \\ strip_tac \\
+
+ drule_strip (SIMP_RULE (srw_ss()) [] INIT_REL_circuit_verilog) \\
+ pop_assum(qspec_then`k1`strip_assume_tac) \\
+ qexists_tac `m` \\ rpt strip_tac' \\
+
+ fs [is_lab_env_def] \\
+ drule_strip is_mem_verilog \\
+ drule_strip is_interrupt_interface_verilog \\
+ drule_strip (SIMP_RULE (srw_ss()) [] circuit_halt_compute_step_full_actual') \\
+ fs [arithmeticTheory.LESS_EQ_EXISTS] \\
+ qmatch_assum_rename_tac `k = m + m1` \\ rveq \\
+ disch_then (qspecl_then [`m`, `m1`] mp_tac) \\ impl_tac
+ >- (rpt conj_tac
+    >- (fs [REL_def] \\
+       CONV_TAC (RAND_CONV (REWRITE_CONV [readerCompileTheory.config_def] THENC EVAL)) \\
+       EVAL_TAC)
+    >- rfs [REL_def, get_mem_word_word_at_addr]
+    \\ fs [halt_inv_def, REL_def]) \\
+ strip_tac \\
+
+ drule_strip computer_Next_relM_run \\ pop_assum (qspec_then `m1 + m` strip_assume_tac) \\
+ fs [REL_def, is_halted_def, ag32_machine_configTheory.ag32_machine_config_def] \\
+
+(* lift_tac 2
+          cake_ag32_next
+          ag32BootstrapTheory.config_def \\*)
+
+ (* End of lift_tac *)
+ drule_strip (reader_extract_writes |> GEN_ALL) \\
+ pop_assum (qspecl_then [`mem`, `input`] mp_tac) \\
+ simp [] \\
+ qunabbrev_tac `res` \\
+ TOP_CASE_TAC \\ strip_tac \\
+ rpt conj_tac
+
+ >- (every_case_tac \\ fs [relM_def, relM_var_def, WORD_def])
+
+ >- (fs [relM_def, relM_var_def, WORD_def])
+
+ >- (every_case_tac \\ metis_tac [is_prefix_extract_writes])
+
+ >- (every_case_tac \\ metis_tac [is_prefix_extract_writes])
+
+ \\ strip_tac \\ rfs [] \\ drule_strip after_R_1w_lift \\ drule_first \\
+    every_case_tac \\ fs [reader_extract_writes]);
+
+val _ = save_thm("reader_ag32_next_verilog",
+ reader_ag32_next_verilog |> REWRITE_RULE [LET_THM] |> BETA_RULE);
 
 val _ = export_theory ();
