cakeml_connection/sortVerilogProofScript.sml
@@ -1,0 +1,97 @@
+open hardwarePreamble;
+
+open sortProofTheory;
+
+open commonVerilogProofLib;
+
+val _ = new_theory "sortVerilogProof";
+
+val sort_spec_def = Define `
+ sort_spec input output <=>
+  ?output'.
+   output = explode (concat output') /\
+   PERM output' (lines_of (implode input)) /\
+   SORTED mlstring_le output'`;
+
+(* Another case where lift_tac is not general enough *)
+
+val sort_ag32_next_verilog_lem = Q.prove(
+ `!vstep fext ms input.
+   vstep = verilog_sem fext computer ms ∧
+
+   STRLEN input ≤ stdin_size ∧
+   is_lab_env fext_accessor_verilog vstep fext ∧
+   ag32_verilog_init (code, data, config) ([strlit "sort"], input) ms fext
+   ⇒
+   ?k1. !k. k1 ≤ k ==> ?fin.
+    vstep k = INR fin /\
+    let stdout = extract_writes 1 (MAP get_ag32_io_event (fext k).io_events);
+        stdout_spec = extract_writes 1 (MAP get_output_io_event (sort_io_events input))
+    in
+      is_halted (code, data, config) fin ∧
+      stdout ≼ stdout_spec ∧
+      (exit_code_0 fin ⇒ stdout = stdout_spec)`,
+ rewrite_tac [verilog_sem_def] \\ rpt gen_tac \\
+ SELECT_ELIM_TAC \\ conj_tac >- metis_tac[lift_fext_exists] \\
+
+ rewrite_tac [ag32_verilog_init_def] \\ rpt strip_tac \\
+ drule_strip (vars_has_type_append |> SPEC_ALL |> EQ_IMP_RULE |> fst |> SPEC_ALL) \\
+
+ drule_strip relM_backwards \\
+ drule_strip INIT_backwards \\
+ qmatch_asmsub_abbrev_tac `INIT _ _ s'` \\
+
+ drule_strip (sort_ag32_next |> GEN_ALL) \\
+
+ disch_then (qspec_then `s'` mp_tac) \\
+ impl_tac >- (qunabbrev_tac `s'` \\ simp [ag32_targetTheory.is_ag32_init_state_def]) \\
+
+ strip_tac \\
+ first_x_assum(qspec_then`k1`mp_tac) \\
+ impl_tac >- simp[] \\ strip_tac \\
+
+ drule_strip (SIMP_RULE (srw_ss()) [] INIT_REL_circuit_verilog) \\
+ pop_assum(qspec_then`k1`strip_assume_tac) \\
+ qexists_tac `m` \\ rpt strip_tac' \\
+
+ fs [is_lab_env_def] \\
+ drule_strip is_mem_verilog \\
+ drule_strip is_interrupt_interface_verilog \\
+ drule_strip (SIMP_RULE (srw_ss()) [] circuit_halt_compute_step_full_actual') \\
+ fs [arithmeticTheory.LESS_EQ_EXISTS] \\
+ qmatch_assum_rename_tac `k = m + m1` \\ rveq \\
+ disch_then (qspecl_then [`m`, `m1`] mp_tac) \\ impl_tac
+ >- (rpt conj_tac
+    >- (fs [REL_def] \\
+       CONV_TAC (RAND_CONV (REWRITE_CONV [sortCompileTheory.config_def] THENC EVAL)) \\
+       EVAL_TAC)
+    >- rfs [REL_def, get_mem_word_word_at_addr]
+    \\ fs [halt_inv_def, REL_def]) \\
+ strip_tac \\
+
+ drule_strip computer_Next_relM_run \\ pop_assum (qspec_then `m1 + m` strip_assume_tac) \\
+ fs [REL_def, is_halted_def, ag32_machine_configTheory.ag32_machine_config_def] \\
+
+ (* Overkill: *)
+ lift_stdout_tac sort_extract_writes_stdout);
+
+val sort_ag32_next_verilog = Q.store_thm("sort_ag32_next_verilog",
+ `!vstep fext ms input.
+   vstep = verilog_sem fext computer ms ∧
+
+   STRLEN input ≤ stdin_size ∧
+   is_lab_env fext_accessor_verilog vstep fext ∧
+   ag32_verilog_init (code, data, config) ([strlit "sort"], input) ms fext
+   ⇒
+   ?output. ?k1. !k. k1 ≤ k ==> ?fin.
+    sort_spec input output /\
+    vstep k = INR fin /\
+    let stdout = extract_writes 1 (MAP get_ag32_io_event (fext k).io_events);
+    in
+      is_halted (code, data, config) fin ∧
+      stdout ≼ output ∧
+      (exit_code_0 fin ⇒ stdout = output)`,
+ rewrite_tac [sort_spec_def] \\
+ metis_tac [sort_ag32_next_verilog_lem, sort_extract_writes_stdout]);
+
+val _ = export_theory ();
